\documentclass[aip,jcp,reprint,amsmath,amssymb,floatfix,citeautoscript,nofootinbib,onecolumn]{revtex4-2}
%\documentclass[aps,prx,reprint,amsmath,amssymb,floatfix,citeautoscript,superscriptaddress]{revtex4-1}
%\documentclass{article}
\usepackage{cancel}
\usepackage{amsmath}
\usepackage{physics}
\usepackage{graphicx}
\usepackage{amssymb}
\usepackage{amsthm}
\usepackage{mathrsfs}
\usepackage{bm}
\usepackage{dcolumn}% Align table columns on decimal point
\newcolumntype{x}[1]{D{.}{.}{#1}}

\usepackage{ragged2e}
\usepackage{txfonts}
\allowdisplaybreaks

\usepackage{color}
\usepackage[usenames,dvipsnames]{xcolor}
\definecolor{myblue}{rgb}{0,0,1}
\usepackage[breaklinks=true,colorlinks=true,linkcolor=myblue,urlcolor=myblue,citecolor=myblue]{hyperref}
\newcommand{\red}[1]{{\color[rgb]{0.6,0,0}{#1}}}
\newcommand{\green}[1]{{\color[rgb]{0,0.6,0}{#1}}}

\newcommand{\vk}{{\bm{k}}}
\newcommand{\vG}{{\bm{G}}}

\begin{document}

\section{CCSD}

Defining some quantities

ERIs, which notation?
\begin{equation}
    v^{pr}_{qs}=\left(pq|rs\right)
\end{equation}

\begin{equation}
    w^{ij}_{ab}=2v^{ij}_{ab}-v^{ij}_{ba}
\end{equation}

CCSD energy equation
\begin{equation}
    E=\ev{He^{T_1+T_2}}{\Phi_0}
\end{equation}

\begin{equation}
    E_\mathrm{CCSD} = 2\sum_{i,a}f^i_at^a_i+\sum_{i,j,a,b}w^{ij}_{ab}t^a_it^b_j+\sum_{i,j,a,b}w^{ij}_{ab}t^{ab}_{ij}
\end{equation}

Defining the $T_1$ transformed operators
\begin{equation}
    \hat{O}=e^{-T_1}Oe^{T_1}
\end{equation}

The CCSD amplitude equations with transformed operators
\begin{gather}
    \mel{\Phi^a_i}{\hat{H}+\left[\hat{H},T_2\right]}{\Phi_0}=0\\
    \mel{\Phi^{ab}_{ij}}{\hat{H}+\left[\hat{H},T_2\right]+\frac{1}{2}\left[\left[\hat{H},T_2\right],T_2\right]}{\Phi_0}=0
\end{gather}

$T_1$ amplitude equation
\begin{equation}
    \begin{aligned}
        0=&f^a_i-2\sum_{k,c}f^k_ct^a_kt^c_i+\sum_c\kappa^a_ct^c_i-\sum_k\kappa^k_it^a_k\\
        &+\sum_{k,c}\kappa^k_c\left(2t^{ca}_{ki}-t^{ca}_{ik}\right)+\sum_{k,c}\kappa^k_ct^c_it^a_k+\sum_{k,c}w^{ak}_{ic}t^c_k\\
        &+\sum_{k,c,d}w^{ak}_{cd}t^{cd}_{ik}+\sum_{k,c,d}w^{ak}_{cd}t^c_it^d_k-\sum_{k,l,c}w^{kl}_{ic}t^{ac}_{kl}\\
        &-\sum_{k,l,c}w^{kl}_{ic}t^a_kt^c_l
    \end{aligned}
\end{equation}

$T_2$ Amplitude Equations
\begin{equation}
    \begin{aligned}
        0=&v^{ij}_{ab}+\sum_{k,l}\chi^{kl}_{ij}t^{ab}_{kl}+\sum_{k,l}\chi^{kl}_{ij}t^a_kt^b_l+\sum_{c,d}\chi^{ab}_{cd}t^{cd}_{ij}\\
        &+\sum_{c,d}\chi^{ab}_{cd}t^c_it^d_j+P\sum_c\lambda^a_ct^{cb}_{ij}-P\sum_k\lambda^k_it^{ab}_{kj}\\
        &+P\sum_c\left(v^{ab}_{ic}-\sum_kv^{kb}_{ic}t^a_k\right)t^c_j-P\sum_k\left(v^{ak}_{ij}+\sum_cv^{ak}_{ic}t^c_j\right)t^b_k\\
        &+P\sum_{k,c}\left(2\chi^{ak}_{ic}-\chi^{ak}_{ci}\right)t^{cb}_{kj}-P\sum_{k,c}\chi^{ak}_{ic}t^{bc}_{kj}\\
        &-P\sum_{k,c}\chi^{bk}_{ci}t^{ac}_{kj}
    \end{aligned}
\end{equation}

Intermediates
\begin{align}
    \kappa^k_i=&f^k_i+\sum_{l,c,d}w^{kl}_{cd}t^{cd}_{il}+\sum_{l,c,d}w^{kl}_{cd}t^c_it^d_l\\
    \kappa^a_c=&f^a_c-\sum_{k,l,d}w^{kl}_{cd}t^{ad}_{kl}-\sum_{k,l,d}w^{kl}_{cd}t^a_kt^d_l\\
    \kappa^k_c=&f^k_c+\sum_{l,d}w^{kl}_{cd}t^d_l\\
    \lambda^k_i=&\kappa^k_i+\sum_cf^k_ct^c_i+\sum_{l,c}w^{kl}_{ic}t^c_l\\
    \lambda^a_c=&\kappa^a_c-\sum_kf^k_ct^a_k+\sum_{k,d}w^{ak}_{cd}t^d_k\\
    \chi^{kl}_{ij}=&v^{kl}_{ij}+\sum_cv^{kl}_{ic}t^c_j+\sum_cv^{kl}_{cj}t^c_i+\sum_{c,d}v^{kl}_{cd}t^{cd}_{ij}+\sum_{l,d}v^{lk}_{dc}t^d_it^a_l\\
    \chi^{ab}_{cd}=&v^{ab}_{cd}-\sum_kv^{ak}_{cd}t^b_k-\sum_kv^{kb}_{cd}t^a_k\\
    \chi^{ak}_{ic}=&v^{ak}_{ic}-\sum_lv^{lk}_{ic}t^a_l+\sum_dv^{ak}_{dc}t^d_i-\frac{1}{2}\sum_{l,d}v^{lk}_{dc}t^{da}_{il}\\
        &-\sum_{l,d}v^{lk}_{dc}t^d_it^a_l+\frac{1}{2}\sum_{l,d}w^{lk}_{dc}t^{ad}_{il}\notag\\
    \chi^{ak}_{ci}=&v^{aj}_{ci}-\sum_lv^{lk}_{ci}t^a_l+\sum_dv^{ak}_{cd}t^d_i-\frac{1}{2}\sum_{l,d}v^{lk}_{cd}t^{da}_{il}\notag\\
        &-\sum_{l,d}v^{lk}_{cd}t^d_it^a_l
\end{align}

\section{CC2}
The doubles equations are approximated to first order.

The CC2 doubles amplitude equations with transformed operators
\begin{equation}
    \mel{\Phi^{ab}_{ij}}{\left[F,T_2\right]+\hat{H}}{\Phi_0}=0
\end{equation}
Note that $F$ doesn't have a hat!

Current implementation of $T_2$ amplitude equations
\begin{equation}
    \begin{aligned}
        0=&v^{ij}_{ab}+\sum_{k,l}\chi^{kl}_{ij}t^a_kt^b_l+\sum_{c,d}\chi^{ab}_{cd}t^c_it^d_j+P\sum_c\lambda^a_ct^{cb}_{ij}-P\sum_k\lambda^k_it^{ab}_{kj}\\
        &+P\sum_c\left(v^{ab}_{ic}-\sum_kv^{kb}_{ic}t^a_k\right)t^c_j-P\sum_k\left(v^{ak}_{ij}+\sum_cv^{ak}_{ic}t^c_j\right)t^b_k
    \end{aligned}
\end{equation}

Intermediates
\begin{align}
    \kappa^k_i=&f^k_i\\
    \kappa^a_c=&f^a_c\\
    \lambda^k_i=&\kappa^k_i+\sum_cf^k_ct^c_i\\
    \lambda^a_c=&\kappa^a_c-\sum_kf^k_ct^a_k\\
    \chi^{kl}_{ij}=&v^{kl}_{ij}+\sum_cv^{kl}_{ic}t^c_j+\sum_cv^{kl}_{cj}t^c_i+\sum_{l,d}v^{lk}_{dc}t^d_it^a_l\\
    \chi^{ab}_{cd}=&v^{ab}_{cd}-\sum_kv^{ak}_{cd}t^b_k-\sum_kv^{kb}_{cd}t^a_k\\
\end{align}

$T_1$ transform
\begin{align}
    X_{\alpha i}=&C_{\alpha i}\\
    X_{\alpha a}=&C_{\alpha a}-\sum_iC_{\alpha i}t^a_i\\
    Y_{\alpha i}=&C_{\alpha i}+\sum_aC_{\alpha a}t^a_i\\
    Y_{\alpha a}=&C_{\alpha a}
\end{align}

$T_1$ transformed two-electron integral
\begin{equation}
    \hat{\left(pq|rs\right)}=\sum_{\mu\nu\lambda\sigma}X_{\mu p}Y_{\nu q}X_{\lambda r}Y_{\sigma s}\left(\mu\nu|\lambda\sigma\right)
\end{equation}

Doubles amplitude
\begin{equation}
    t^{ab}_{ij}=\frac{\hat{\left(ai|bj\right)}}{\varepsilon_i-\varepsilon_a+\varepsilon_j-\varepsilon_b}
\end{equation}


\section{EOMEE}
Original Barlett Paper
\begin{equation}
	\expval{a^\dagger b}=\rho_{ab} = r_0\left[t^b_ml^m_a+\frac{1}{2}t^{eb}_{mn}l^{mn}_{ea}\right] + r^b_ml^m_a+\frac{1}{2}r^{eb}_{mn}l^{mn}_{ea} + t^b_nr^e_ml^{mn}_{ea}
\end{equation}

Krylov dervation
\begin{equation}
	\gamma_{ab}' = \frac{1}{2}P_+(ab)\left(\sum_il^a_i\tilde{\tilde{r}}_{ib}+\tilde{l}^{ab}+\sum_iY^1_{ia}t^b_i\right)
\end{equation}

\begin{equation}
	\tilde{\tilde{r}}_{ib}=r^b_i+r_0t^b_i
\end{equation}

\begin{equation}
	\tilde{l}^{ab} = \frac{1}{2}\sum_{ijc}l^{ac}_{ij}\tilde{\tilde{r}}^{bc}_{ij}
\end{equation}

\begin{equation}
	\tilde{\tilde{r}}^{bc}_{ij} = r^{bc}_{ij}+r_0t^{bc}_{ij}
\end{equation}

\begin{equation}
	\gamma_{ab}' = \frac{1}{2}P_+(ab)\left(\sum_il^a_ir^b_i+r_0l^a_it^b_i+\frac{1}{2}l^{ac}_{ij}r^{bc}_{ij}+\frac{1}{2}r_0l^{ac}_{ij}t^{bc}_{ij}+\sum_il^{ab}_{ij}r^b_jt^b_i\right)
\end{equation}

\begin{align}
	\gamma_{ab}' &= \frac{1}{2}\left(\sum_il^a_ir^b_i+r_0l^a_it^b_i+\frac{1}{2}l^{ac}_{ij}r^{bc}_{ij}+\frac{1}{2}r_0l^{ac}_{ij}t^{bc}_{ij}+\sum_il^{ab}_{ij}r^b_jt^b_i\right) \\
	&+\frac{1}{2}\left(\sum_il^b_ir^a_i+r_0l^b_it^a_i+\frac{1}{2}l^{bc}_{ij}r^{ac}_{ij}+\frac{1}{2}r_0l^{bc}_{ij}t^{ac}_{ij}+\sum_il^{ba}_{ij}r^a_jt^a_i\right)
\end{align}

\begin{equation}
	Y^1_{ia} = \sum_{jb}l^{ab}_{ij}r^b_j
\end{equation}

\section{EOMIP}
\begin{equation}
	\gamma_{ab}'=\frac{1}{2}P_+(ab)\left(\tilde{l}^{ab}-\sum_iY^1_{ia}t^b_i\right)
\end{equation}

\begin{equation}
	Y^1_{ia} = \sum_jl^a_{ij}r_j
\end{equation}

\begin{equation}
	\tilde{l}^{ab} = \frac{1}{2}\sum_{ij}l^a_{ij}r^b_{ij}
\end{equation}

\begin{equation}
	\gamma_{ab}'=\frac{1}{2}P_+(ab)\left(\frac{1}{2}\sum_{ij}l^a_{ij}r^b_{ij}-\sum_jl^a_{ij}r_jt^b_i\right)
\end{equation}

\begin{align}
	\gamma_{ab}'&=\frac{1}{2}\left(\frac{1}{2}\sum_{ij}l^a_{ij}r^b_{ij}-\sum_{ij}l^a_{ij}r_jt^b_i\right) \\
	&+\frac{1}{2}\left(\frac{1}{2}\sum_{ij}l^b_{ij}r^a_{ij}-\sum_{ij}l^b_{ij}r_jt^a_i\right)
\end{align}

\section{EOMEA}
\begin{equation}
	\gamma_{ab}'=\frac{1}{2}P_+(ab)\left(l^ar^b+\tilde{l}_{ab}\sum_kY^1_{ka}t^b_k\right)
\end{equation}

\begin{equation}
	\tilde{l}_{ab} = \sum_{kc}l^{ac}_kr^{bc}_k
\end{equation}

\begin{equation}
	Y^1_{ka}=\sum_cl^{ac}_kr^c
\end{equation}

\begin{equation}
	\gamma_{ab}' = \frac{1}{2}P_+(ab)\left(\sum_il^ar^b+\frac{1}{2}l^{ac}_{i}r^{bc}_{i}+\sum_ml^{ac}_{k}r^ct^b_k\right)
\end{equation}

\begin{align}
	\gamma_{ab}' &= \frac{1}{2}\left(\sum_il^ar^b+\frac{1}{2}l^{ac}_{i}r^{bc}_{i}+\sum_kl^{ac}_{k}r^ct^b_k\right) \\
	&+\frac{1}{2}\left(\sum_il^br^a+\frac{1}{2}l^{bc}_ir^{ac}_i+\sum_il^{bc}_kr^ct^a_k\right)
\end{align}
\end{document}
